Optimizations/Canonicalizations/TacticSolving.thy
@@ -114,7 +114,7 @@ lemma exp_xor_self_is_false:
   shows "exp[x \<oplus> x] >= exp[false]"
   unfolding le_expr_def using assms unfolding wf_stamp_def
   using val_xor_self_is_false evaltree_not_undef
-  by (smt (z3) bin_eval.simps(6) bin_eval_new_int constantAsStamp.simps(1) evalDet int_signed_value_bounds new_int.simps new_int_take_bits unfold_binary unfold_const valid_int valid_stamp.simps(1) valid_value.simps(1) well_formed_equal_defn)
+  by (smt (z3) wf_value_def bin_eval.simps(6) bin_eval_new_int constantAsStamp.simps(1) evalDet int_signed_value_bounds new_int.simps new_int_take_bits unfold_binary unfold_const valid_int valid_stamp.simps(1) valid_value.simps(1) well_formed_equal_defn)
 
 
 lemma val_or_commute[simp]:
@@ -146,7 +146,7 @@ optimization OrInverse: "exp[n | ~n] \<longmapsto> (const (new_int 32 (not 0)))
                         when (stamp_expr n = IntegerStamp 32 l h \<and> wf_stamp n)"
   unfolding size.simps apply (simp add: Suc_lessI)
   apply auto using OrInverseVal unfolding wf_stamp_def
-  by (smt (z3) constantAsStamp.simps(1) evalDet int_signed_value_bounds mask_eq_take_bit_minus_one 
+  by (smt (z3) wf_value_def constantAsStamp.simps(1) evalDet int_signed_value_bounds mask_eq_take_bit_minus_one 
       new_int.elims new_int_take_bits unfold_const valid_int valid_stamp.simps(1) 
       valid_value.simps(1) well_formed_equal_defn)
 
@@ -168,7 +168,7 @@ optimization XorInverse: "exp[n \<oplus> ~n] \<longmapsto> (const (new_int 32 (n
                         when (stamp_expr n = IntegerStamp 32 l h \<and> wf_stamp n)"
   unfolding size.simps apply (simp add: Suc_lessI)
   apply auto using XorInverseVal
-  by (smt (verit) constantAsStamp.simps(1) evalDet int_signed_value_bounds intval_xor.elims 
+  by (smt (verit) wf_value_def constantAsStamp.simps(1) evalDet int_signed_value_bounds intval_xor.elims 
       mask_eq_take_bit_minus_one new_int.elims new_int_take_bits unfold_const valid_stamp.simps(1) 
       valid_value.simps(1) well_formed_equal_defn wf_stamp_def)
 
